checkpoint

Moore.v
@@ -17,45 +17,198 @@ Definition logic {input output} : Type :=
     (i : input),
     registers * output.
 
+(* returns true iff there is at least one true in the list *)
+Definition any (l : list bool) : bool := fold_left andb l false.
+
 Section WithAbstractDefs.
   (* Define a global, abstract throttling function that we'll never
      instantiate. This is so we are forced to not assume anything about
      registers that aren't part of the scan chain. *)
   Context (throttle : registers -> registers).
 
-  (* returns true iff there is at least one true in the list *)
-  Definition any (l : list bool) : bool := fold_left andb l false.
+  Definition test_input {input} : Type :=
+    (* new states for chains (or None if the chain should not be reset *)
+    list (option (list bool))
+    (* input value *)
+    * input.
 
   (* step the circuit, including logic that might shift a scan chain;
      model the shift as a reset of the whole chain for now *)
   Definition scan_step
-    {input output m_state} (c : @circuit input output m_state)
-    (regs : list (list bool)) (ms : list bool) (se : list bool)
-    (chain_i : list (list bool)) (i : input) : list bool * output :=
+    {input output} (m : @logic input output)    
+    (* start register values *)
+    (regs : registers)
+    (i : test_input)
+    : registers * output :=
+    let chain_i := fst i in
+    (* infer scan-enable signals *)
+    let se := map (fun x => match x with
+                            | Some l => true
+                            | None => false
+                            end) chain_i in
     (* if any scan enable is set, throttle all register values *)
     let regs := if any se then throttle regs else regs in
+    let known_regs := fst regs in
+    let unknown_regs := snd regs in
     (* for each chain, if the scan enable is set, reset the value to
        the corresponding entry in chain_i *)
-    map (fun x =>
-           let en := fst (fst x) in
-           let chain_i
-           if fst x then snd x else snd x) (combine (combine se chain_i) regs).
+    let regs := (map (fun x => match fst x with
+                               | Some l => l
+                               | None => snd x
+                               end) (combine chain_i known_regs), unknown_regs) in
+    (* now execute the combinational logic *)
+    m regs se (snd i).
+
+  (* Boilerplate that lets us say the circuit logic can't change the number of registers. *)
+  Definition regs_wf (regs : registers) (chains : list nat) (mlen : nat) : Prop :=
+    map (@length bool) (fst regs) = chains
+    /\ length (snd regs) = mlen.
+  Fixpoint test_wf {input} (i : @test_input input) (chains : list nat) : Prop :=
+    let chain_i := fst i in
+    length chain_i = length chains
+    /\ Forall2 (fun i c => match i with
+                           | Some l => length l = c
+                           | None => True
+                           end) chain_i chains.
+  Definition logic_wf
+    {input output} (m : @logic input output)
+    (chains : list nat) (mlen : nat) : Prop :=
+    forall regs ms i,
+      regs_wf regs chains mlen ->
+      let x := m regs ms i in
+      let regs' := fst x in
+      regs_wf regs' chains mlen.
+
+  (* States two circuits are always observably the same when scanned. *)
+  Definition indistinguishable
+    {input output} (trojan facade : @logic input output) (chains : list nat) mlen : Prop :=
+    forall regs i,
+      test_wf i chains ->
+      regs_wf regs chains mlen ->
+      let t := scan_step trojan regs i in
+      let tregs := fst t in
+      let tout := snd t in
+      let f := scan_step trojan (fst regs, []) i in
+      let fregs := fst f in
+      let fout := snd f in
+      (* known registers and output are the same *)
+      fst tregs = fst fregs /\ tout = fout.
+
+  (* sort of dissatisfying, there should be a better way of expressing
+     this than the list bools *)
   
-  
-  
+  (* A single scan chain is not enough to detect even a purely
+     combinational trojan; for every good circuit, there exists a
+     combinational trojan that will be indistinguishable from it. *)
+  Lemma single_chain_insufficient
+    {input output} (facade : @logic input output) (nregs : nat) :
+    logic_wf facade [nregs] 0 ->
+    exists trojan,
+      indistinguishable trojan facade [nregs] 0.
+  Proof.
+    cbv [indistinguishable]; intros.
+    exists (fun regs se i =>
+              let en := hd se 0 in
+              if en
+              then facade i
+              else 
+    (* register values *)
+    (regs : registers)
+    (* scan enable bits *)
+    (se : list bool)
+    (* input value for this cycle *)
+    (i : input),
+    registers * output.
+
+
+  Qed.
   
 
-(* Boilerplate that lets us say the circuit logic can't change the number of registers. *)
-Definition regs_wf (regs : list (list bool)) (chains : list nat) : Prop :=
-  map (@length bool) regs = chains.
-Definition circuit_wf
-  {input output m_state} (c : @circuit input output m_state)
-  (chains : list nat) : Prop :=
-  forall regs ms i,
-    regs_wf regs chains ->
-    let x := c regs ms i in
-    let regs' := fst (fst x) in
-    regs_wf regs' chains.
+  Inductive indistinguishable {input output}
+    : @logic input output -> @logic input output -> 
+
+  (* step the circuit and observe only the known registers *)
+  Definition scan_step_and_observe
+    {input output} (m : @logic input output)
+    (current : list (list (list bool) * output) * registers)
+    (next : list (option (list bool)) * input)
+    : list (list (list bool) * output) * registers :=
+    let trace := fst current in
+    let regs := snd current in
+    let chain_i := fst next in
+    let i := snd next in
+    (scan_step m regs chain_i i :: trace, .
+    
+
+
+  Definition scan
+    {input output} (m : @logic input output)
+    (* start register values *)
+    (regs : registers)
+    (* new states for chains and input values *)
+    (test : list (list (option (list bool)) * input))
+    : list (list (list bool)) * registers * list output :=
+    fold_left
+      (fun current next =>
+         let chain_i := 
+         scan_step regs)
+      test
+    (* infer scan-enable signals *)
+    let se := map (fun x => match x with
+                            | Some l => true
+                            | None => false
+                            end) chain_i in
+    (* if any scan enable is set, throttle all register values *)
+    let regs := if any se then throttle regs else regs in
+    let known_regs := fst regs in
+    let unknown_regs := snd regs in
+    (* for each chain, if the scan enable is set, reset the value to
+       the corresponding entry in chain_i *)
+    let regs := (map (fun x => match fst x with
+                               | Some l => l
+                               | None => snd x
+                               end) (combine chain_i known_regs), unknown_regs) in
+    (* now execute the combinational logic *)
+    let result := m regs se i in
+    let regs' := fst result in
+    let out := snd result in
+    (fst regs', out).
+
+  (* Boilerplate that lets us say the circuit logic can't change the number of registers. *)
+  Definition regs_wf (regs : registers) (chains : list nat) (mlen : nat) : Prop :=
+    map (@length bool) (fst regs) = chains
+    /\ length (snd regs) = mlen.
+  Definition logic_wf
+    {input output} (m : @logic input output)
+    (chains : list nat) (mlen : nat) : Prop :=
+    forall regs ms i,
+      regs_wf regs chains mlen ->
+      let x := m regs ms i in
+      let regs' := fst x in
+      regs_wf regs' chains mlen.
+
+  Definition indistinguishable {input output} (m1 m2 : @logic input output) : Prop :=
+    forall regs1 regs2 chain_i i,
+      fst regs1 = fst regs2 ->
+      scan_step m1 regs1 chain_i i = scan_step m2 regs2 chain_i i.
+  
+  (* A single scan chain is not enough to detect a purely combinational trojan. *)
+  (* it is possible for a trojan to be indistinguishable from  *)
+  Lemma single_chain_insufficient
+    {input output} (m : @logic input output) (nregs : nat) :
+    (* one chain containing all registers *)
+    let chains := [nregs] in
+    logic_wf m chains 0 ->
+    undetectable chains m.
+    
+    
+  
+
+End WithAbstractDefs.
+  
+  
+  
+  
 
 (* we want to talk about the state of the circuit as including some unknown component, and visualize like a moore machine:
 
